Added a bunch of stuff to the Hoare logic section and several supporting laws.

theories/models/utp_basic_model.thy
@@ -1,80 +1,209 @@
 theory utp_basic_model
 imports 
-  "../core/utp_value"
-  "../core/utp_sorts"
+  Derive
+  "../utp_base"
 begin
 
-datatype BV = IntV int | BoolV bool
+default_sort type
 
-instantiation BV :: VALUE
+datatype bval = IntV int | BoolV bool | ListV "bval list"
+
+derive linorder bval
+
+datatype btyp = BoolT | IntT | ListT btyp
+
+derive countable btyp
+
+type_synonym 'a bexp   = "('a, bval) WF_PEXPRESSION"
+type_synonym bpred     = "bval WF_PREDICATE" 
+type_synonym 'a bvar   = "('a, bval) PVAR"
+
+translations
+  (type) "'a bexp" <= (type) "('a, bval) WF_PEXPRESSION"
+  (type) "bpred" <= (type) "bval WF_PREDICATE"
+  (type) "'a bvar" <= (type) "('a, bval) PVAR"
+
+inductive bval_type_rel :: "bval \<Rightarrow> btyp \<Rightarrow> bool" (infix ":\<^sub>b" 50) where
+BoolV_type [intro]: "BoolV x :\<^sub>b BoolT" |
+IntV_type  [intro]: "IntV x :\<^sub>b IntT" |
+ListV_type [intro]: "\<forall> x\<in>set xs. x :\<^sub>b t \<Longrightarrow> ListV xs :\<^sub>b ListT t"
+
+inductive_cases
+  BoolV_cases [elim]: "BoolV x :\<^sub>b t" and
+  BoolT_cases [elim!]: "x :\<^sub>b BootT" and
+  IntV_cases [elim]: "IntV x :\<^sub>b t" and
+  IntT_cases [elim!]: "x :\<^sub>b IntT" and
+  ListV_cases [elim]: "ListV xs :\<^sub>b t" and
+  ListT_cases [elim!]: "x :\<^sub>b ListT a"
+
+instantiation bval :: DEFINED
 begin
 
-fun utype_rel_BV :: "BV \<Rightarrow> nat \<Rightarrow> bool" where
-"utype_rel_BV (IntV n) 0 = True" |
-"utype_rel_BV (BoolV x) (Suc 0) = True" |
-"utype_rel_BV _ _ = False"
+definition "Defined_bval (x::bval) = True"
 
-definition Defined_BV :: "BV \<Rightarrow> bool" where
-"Defined_BV x = True"
+instance ..
+end
+
+declare Defined_bval_def [simp]
+
+instantiation bval :: VALUE
+begin
+
+definition utype_rel_bval :: "bval \<Rightarrow> nat \<Rightarrow> bool" where
+"utype_rel_bval x t \<longleftrightarrow> (\<exists> a. t = to_nat a \<and> x :\<^sub>b a)"
 
 instance
   apply (intro_classes)
-  apply (rule_tac x="0" in exI, rule_tac x = "IntV 1" in exI)
-  apply (simp add:Defined_BV_def)
+  apply (simp add:utype_rel_bval_def)
+  apply (rule_tac x="IntV 0" in exI)
+  apply (auto)
 done
 end
 
-definition "IntT = Abs_UTYPE 0"
-definition "BoolT = Abs_UTYPE 1"
+lemma prjTYPE_inv_bty [simp]
+  : "embTYPE ((prjTYPE t) :: btyp) = (t :: bval UTYPE)"
+  by (metis Rep_UTYPE_elim Rep_UTYPE_inverse embTYPE_def from_nat_to_nat prjTYPE_def utype_rel_bval_def)
 
-lemma IntV_utype [typing]:
-  "IntV n :\<^sub>u 0"
-  by (simp)
+lemma embTYPE_inv_bty [simp]:
+  "prjTYPE (embTYPE (t :: btyp) :: bval UTYPE) = t"
+  apply (induct t)
+  apply (rule embTYPE_inv[of "BoolV False"])
+  apply (auto simp add: utype_rel_bval_def)
+  apply (rule embTYPE_inv[of "IntV 0"])
+  apply (auto simp add: utype_rel_bval_def)
+  apply (rule embTYPE_inv[of "ListV []"])
+  apply (auto simp add: utype_rel_bval_def)
+done
 
-lemma IntV_defined [defined]:
-  "\<D> (IntV n)"
-  by (simp add:Defined_BV_def)
+lemma type_rel_btyp [simp]: 
+  "x : t \<longleftrightarrow> x :\<^sub>b prjTYPE t"
+  by (metis (full_types) Rep_UTYPE_elim empty_Collect_eq from_nat_to_nat prjTYPE_def type_rel_def utype_rel_bval_def)
 
-lemma IntV_type [typing]:
-  "IntV n : IntT"
-  by (simp add: IntT_def type_rel_def Abs_UTYPE_inv[OF IntV_utype IntV_defined])
-
-lemma BoolV_utype [typing]:
-  "BoolV n :\<^sub>u (Suc 0)"
-  by (simp)
-
-lemma BoolV_defined [defined]:
-  "\<D> (BoolV n)"
-  by (simp add:Defined_BV_def)
-
-lemma BoolV_type [typing]:
-  "BoolV n : BoolT"
-  by (simp add: BoolT_def type_rel_def Abs_UTYPE_inv[OF BoolV_utype BoolV_defined])
-
-instantiation BV :: BOOL_SORT
+instantiation bval :: BOOL_SORT
 begin
 
-definition MkBool_BV :: "bool \<Rightarrow> BV" where
-"MkBool_BV x = BoolV x"
+definition MkBool_bval :: "bool \<Rightarrow> bval" where
+"MkBool_bval x = BoolV x"
 
-primrec DestBool_BV :: "BV \<Rightarrow> bool" where
-"DestBool_BV (BoolV x) = x" 
+primrec DestBool_bval :: "bval \<Rightarrow> bool" where
+"DestBool_bval (BoolV x) = x" 
 
-definition BoolType_BV :: "BV UTYPE" where
-"BoolType_BV = Abs_UTYPE 1"
+definition BoolType_bval :: "bval UTYPE" where
+"BoolType_bval = embTYPE BoolT"
 
 instance
   apply (intro_classes)
-  apply (simp add:MkBool_BV_def DestBool_BV_def BoolType_BV_def dcarrier_def monotype_def Defined_BV_def type_rel_def)
-  apply (simp add:MkBool_BV_def DestBool_BV_def BoolType_BV_def dcarrier_def monotype_def Defined_BV_def type_rel_def)
-  apply (simp add: Abs_UTYPE_inv[OF BoolV_utype BoolV_defined])
-  apply (auto simp add:MkBool_BV_def)
-  apply (case_tac x)
-  apply (simp)
-  apply (simp add:image_def MkBool_BV_def)
-  apply (auto simp add:monotype_def BoolType_BV_def Abs_UTYPE_inv[OF BoolV_utype BoolV_defined] type_rel_def)
-  apply (case_tac x)
-  apply (auto)
-  apply (metis (full_types) list_decode.cases utype_rel_BV.simps(3) utype_rel_BV.simps(6))
+  apply (simp add:MkBool_bval_def DestBool_bval_def BoolType_bval_def dcarrier_def monotype_def Defined_bval_def type_rel_def)
+  apply (auto simp add:MkBool_bval_def DestBool_bval_def BoolType_bval_def Defined_bval_def dcarrier_def monotype_def)
+  apply (metis prjTYPE_inv_bty)
 done
+end
+
+instantiation bval :: INT_SORT
+begin
+
+definition MkInt_bval :: "int \<Rightarrow> bval" where
+"MkInt_bval x = IntV x"
+
+primrec DestInt_bval :: "bval \<Rightarrow> int" where
+"DestInt_bval (IntV x) = x" 
+
+definition IntType_bval :: "bval UTYPE" where
+"IntType_bval = embTYPE IntT"
+
+instance
+  apply (intro_classes)
+  apply (simp add:MkInt_bval_def DestInt_bval_def IntType_bval_def dcarrier_def monotype_def Defined_bval_def type_rel_def)
+  apply (auto simp add:MkInt_bval_def DestInt_bval_def IntType_bval_def Defined_bval_def dcarrier_def monotype_def)
+done
+end
+
+syntax
+  "_pexpr_op1" :: "idt \<Rightarrow> pexpr \<Rightarrow> pexpr" ("_'(_')")
+  "_pexpr_op2" :: "idt \<Rightarrow> pexpr \<Rightarrow> pexpr \<Rightarrow> pexpr" ("_'(_,_')")
+
+translations
+  "_pexpr_op1 f x"   == "CONST Op1PE f x"
+  "_pexpr_op2 f x y" == "CONST Op2PE f x y"
+
+term "|x > y|"
+
+term "`X := $X - $Y \<lhd> ($X > $Y) \<rhd> Y := $Y - $X`"
+
+term "MkPlainP n True t TYPE(bval)"
+
+abbreviation MkV :: "string \<Rightarrow> 'a itself \<Rightarrow> 'a bvar" where
+"MkV n t \<equiv> MkPlainP n True t TYPE(bval)"
+
+abbreviation "X \<equiv> MkV ''X'' TYPE(int)"
+abbreviation "Y \<equiv> MkV ''Y'' TYPE(int)"
+
+abbreviation "GCD_BODY \<equiv> `X := $X - $Y \<lhd> $X > $Y \<rhd> Y := $Y - $X`"
+
+abbreviation 
+"GCD \<equiv> `while \<not>($X = $Y) do GCD_BODY od`"
+
+abbreviation
+  "GCD_INV x y \<equiv> `($X > \<guillemotleft>0\<guillemotright>) \<and> ($Y > \<guillemotleft>0\<guillemotright>) \<and> (gcd($X,$Y) = gcd(\<guillemotleft>x\<guillemotright>,\<guillemotleft>y\<guillemotright>))`"
+
+lemma GCD_pre_sat_GCD_INV:
+  "\<lbrakk> x > 0; y > 0 \<rbrakk> \<Longrightarrow> `($X > \<guillemotleft>0\<guillemotright>) \<and> ($Y > \<guillemotleft>0\<guillemotright>) \<and> (gcd($X,$Y) = gcd(\<guillemotleft>x\<guillemotright>,\<guillemotleft>y\<guillemotright>))` \<sqsubseteq> `($X = \<guillemotleft>x\<guillemotright> \<and> $Y = \<guillemotleft>y\<guillemotright>)`"
+  by (utp_pred_auto_tac)
+
+lemma GCD_post_sat_GCD_INV:
+  "\<lbrakk> x > 0; y > 0 \<rbrakk> \<Longrightarrow> `($X > \<guillemotleft>0\<guillemotright>) \<and> ($Y > \<guillemotleft>0\<guillemotright>) \<and> (gcd($X,$Y) = gcd(\<guillemotleft>x\<guillemotright>,\<guillemotleft>y\<guillemotright>))` \<sqsubseteq> `$X = $Y \<and> $X = gcd(\<guillemotleft>x\<guillemotright>,\<guillemotleft>y\<guillemotright>)`"
+  apply (utp_pred_auto_tac)
+  apply (metis gcd_pos_int less_int_code(1))
+  apply (metis abs_gcd_int)
+done
+
+theorem GCD_partial_correct:
+  assumes "x > 0" "y > 0"
+  shows "`($X = \<guillemotleft>x\<guillemotright> \<and> $Y = \<guillemotleft>y\<guillemotright>){GCD}($X = $Y \<and> $X = gcd(\<guillemotleft>x\<guillemotright>,\<guillemotleft>y\<guillemotright>))`"
+proof -
+  let ?I = "GCD_INV x y" and ?S = "`\<not> ($X = $Y)`"
+
+  have "?I {while ?S do GCD_BODY od}\<^sub>p (\<not>\<^sub>p ?S \<and>\<^sub>p ?I)"
+    apply (rule_tac HoareP_IterP)
+    apply (force intro:closure unrest simp add:erasure typing)
+    apply (force intro:closure unrest simp add:erasure typing)
+    apply (rule closure)
+    apply (force intro:closure unrest simp add:erasure typing defined)+
+    apply (rule HoareP_CondR)
+    apply (rule HoareP_AssignR)
+    apply (force intro:closure unrest simp add:erasure typing defined)
+    apply (simp add:usubst typing defined)
+    apply (utp_pred_auto_tac)
+    apply (smt gcd_add1_int)
+    apply (smt gcd_add1_int)
+    apply (simp add:closure)
+    apply (simp add:closure unrest typing)
+    apply (simp add:closure typing defined)
+    apply (rule HoareP_AssignR)
+    apply (force intro:closure unrest simp add:erasure typing defined)+
+    apply (simp add:usubst typing defined)
+    apply (utp_pred_auto_tac)
+    apply (smt gcd_add2_int)
+    apply (smt gcd_add2_int)
+    apply (simp add:closure)
+    apply (simp add:unrest closure typing defined)
+    apply (simp add:unrest closure typing defined)
+  done
+
+  moreover from assms 
+  have "`$X = $Y \<and> $X = gcd(\<guillemotleft>x\<guillemotright>,\<guillemotleft>y\<guillemotright>)` \<sqsubseteq> ?I \<and>\<^sub>p `$X = $Y` "
+    by (utp_pred_auto_tac)
+
+  ultimately show ?thesis
+    apply (rule_tac HoareP_post_refine)
+    apply (simp)
+    apply (rule HoareP_pre_refine)
+    apply (rule GCD_pre_sat_GCD_INV)
+    apply (simp_all add:assms)
+    apply (metis AndP_comm)
+  done
+qed
+
+value "gcd (33::int) 12"
+
 end
