theories/core/utp_lattice.thy
@@ -370,14 +370,14 @@ end
 
 lemma SkipR_SupP_def: 
   "II = \<Squnion> { $\<^sub>ex\<acute> ==\<^sub>p $\<^sub>ex | x. x \<in> UNDASHED}"
-  apply (auto simp add:SkipR_def Inf_WF_PREDICATE_def UNDASHED_nempty EqualP_def VarE.rep_eq)
+  apply (auto intro!:destPRED_intro simp add:SkipR_def Inf_WF_PREDICATE_def UNDASHED_nempty EqualP_def VarE.rep_eq)
   apply (metis (lifting, full_types) LiftP.rep_eq destPRED_inverse mem_Collect_eq)
 done
 
 lemma SkipRA_SupP_def: 
   "\<lbrakk> vs \<subseteq> REL_VAR; HOMOGENEOUS vs \<rbrakk> \<Longrightarrow> 
      II\<^bsub>vs\<^esub> = \<Squnion> { $\<^sub>ex\<acute> ==\<^sub>p $\<^sub>ex | x. x \<in> in vs}"
-  apply (auto simp add:SkipRA_rep_eq_alt Inf_WF_PREDICATE_def UNDASHED_nempty EqualP_def VarE.rep_eq top_WF_PREDICATE_def TrueP_def)
+  apply (auto intro!:destPRED_intro simp add:SkipRA_rep_eq_alt Inf_WF_PREDICATE_def UNDASHED_nempty EqualP_def VarE.rep_eq top_WF_PREDICATE_def TrueP_def)
   apply (metis (lifting, full_types) LiftP.rep_eq destPRED_inverse mem_Collect_eq)
 done
 
